

1-  $D = \{(1,2), (2,3), (3,5), (4,4), (5,6)\} \rightarrow (3,4)$

a)  $X = \begin{bmatrix} -2 & -2 \\ -1 & -1 \\ 0 & 1 \\ 1 & 0 \\ 2 & 2 \end{bmatrix} \quad \Sigma = \frac{1}{n-1} X^T X$

$$\Sigma = \frac{1}{4} \begin{bmatrix} 10 & 9 \\ 9 & 10 \end{bmatrix} \quad X^T X = \begin{bmatrix} 10 & 9 \\ 9 & 10 \end{bmatrix}$$

$$\Sigma \gamma_1 = \lambda_1 \gamma_1 \rightarrow (\Sigma - \lambda_1 I) \gamma_1 = 0 \rightarrow \det(\Sigma - \lambda_1 I) = 0$$

$$\lambda_1 = \frac{19}{4} \quad \gamma_1 = (1, 1) \quad \leftarrow \text{PC 1}$$

$$\lambda_2 = \frac{1}{4} \quad \gamma_2 = (-1, 1) \quad \leftarrow \text{PC 2}$$

b)

$$\begin{bmatrix} -2 & -2 \\ -1 & -1 \\ 0 & 1 \\ 1 & 0 \\ 2 & 2 \end{bmatrix} \begin{bmatrix} 1 & 1 \\ +1 & -1 \\ +1 & +1 \end{bmatrix} = \begin{bmatrix} -1 & 0 \\ -2 & 0 \\ +1 & +1 \\ +1 & -1 \\ +4 & 0 \end{bmatrix}$$

c)

$$\frac{\frac{19}{4}}{\frac{19}{4} + \frac{1}{4}} = \frac{19}{20} = 0.95$$

2-  $X = \{x_1, x_2, \dots, x_n\} \quad \gamma_{ij} = \mathbb{1}(x_i \in \text{cluster } j)$

$$\mu_1, \mu_2, \dots, \mu_k$$

$$J = \sum_{j=1}^k \sum_{i=1}^n \gamma_{ij} \|x_i - \mu_j\|^2$$

a) each step: 1 - assignment 2 - update  $J \rightarrow \underline{k^n}$

↳ decreases  $J$   $\leftarrow$

$$b) \quad T = \frac{1}{n} \sum_i \|x_i - \hat{x}\|^2 \quad \hat{x} = \frac{1}{n} \sum_i x_i \quad \rightarrow \text{در میانه کلی}$$

$$\rightarrow W_j(X) = \frac{(\sum_i \gamma_{ij} \|x_i - \mu_j\|^2)}{\sum_i \gamma_{ij}} \quad \rightarrow \text{در میانه درون خوشه‌ها}$$

$$B(X) = \sum_j \left( \frac{\sum_i \gamma_{ij}}{n} \right) \|\mu_j - \hat{x}\|^2 \quad \rightarrow \text{cluster-level distance}$$

$$T = \sum_j \left( \frac{\sum_i \gamma_{ij}}{n} \right) W_j(X) + B(X)$$

$\downarrow \propto J$

$$J = \sum_j \left( \sum_i \gamma_{ij} \|x_i - \mu_j\|^2 \right)$$

$$c) \quad \min J(k) \geq \min J(k+1) \quad k=n \quad J \geq 0$$

$$\gamma_{ij} = I_{n \times n} \rightarrow J=0$$

3-

$$a) \quad P(x, z; \theta) = \underbrace{P(z; \theta)}_{\substack{P(1; \theta) = \pi \\ P(0; \theta) = (1-\pi)}} P(x|z; \theta) = \pi^z (1-\pi)^{(1-z)} P_r^{xz} P_b^{x(1-z)} (1-P_r)^{(1-x)z} (1-P_b)^{(1-x)(1-z)}$$

$$P(z; \theta) = \begin{cases} P(1; \theta) = \pi & z=1 \\ P(0; \theta) = (1-\pi) & z=0 \end{cases} \quad \ln a^b = b \ln a$$

$$b) \quad \mathcal{L}^{(0)} = \sum_{i=1}^m \left[ z_i \ln \pi + (1-z_i) \ln(1-\pi) + x_i z_i \ln P_r + x_i (1-z_i) \ln P_b \right. \\ \left. + (1-x_i) z_i \ln(1-P_r) + (1-x_i)(1-z_i) \ln(1-P_b) \right]$$

$$c) \quad \frac{\partial \mathcal{L}^{(0)}}{\partial \pi} \Big|_{\pi^*} = 0 \rightarrow \pi^* = \frac{\sum_i z_i}{m} \quad P_r^* = \frac{\sum_i x_i z_i}{\sum_i z_i} \quad P_b^* = \frac{\sum_i x_i (1-z_i)}{m - \sum_i z_i}$$

$$\frac{\partial \mathcal{L}}{\partial P_r} \Big|_{P_r^*} = 0 \rightarrow$$

$$\frac{\partial \mathcal{L}}{\partial P_b} \Big|_{P_b^*} = 0 \rightarrow$$

$$d) \quad P(z_i=1 | x_i; \theta^{(t)}) = \frac{P(x_i | z_i=1; \theta^{(t)}) P(z_i=1; \theta^{(t)})}{[P(x_i | z_i=1; \theta^{(t)}) P(z_i=1; \theta^{(t)}) + P(x_i | z_i=0; \theta^{(t)}) P(z_i=0; \theta^{(t)})]} = \checkmark$$

$$= \frac{[P_r^{x_i} (1-P_r^{(t)})^{1-x_i}]}{P_r^{x_i} (1-P_r^{(t)})^{1-x_i} \pi^{(t)} + P_b^{x_i} (1-P_b^{(t)})^{1-x_i} (1-\pi^{(t)})} \quad \checkmark$$

c)  $\mathcal{M} \quad y_i^t = p(z_i = 1 | x_i; \theta^t) \quad Q = E_{z|x, \theta^t} [\ln p(x, z | \theta)]$

$$Q = \sum_{i=1}^m \left( y_i^t \ln p(x_i; z=1; \theta) + (1-y_i^t) \ln p(x_i; z=0; \theta) \right) =$$

$$= \sum_{i=1}^m \left[ y_i^t \left( \ln \pi + x_i \ln p_r + (1-x_i) \ln(1-p_r) \right) + (1-y_i^t) \left( \ln(1-\pi) + x_i \ln p_b + (1-x_i) \ln(1-p_b) \right) \right]$$

$\partial/\partial \pi$ :

$$\sum_{i=1}^m \left( \frac{y_i^t}{\pi} - \frac{(1-y_i^t)}{1-\pi} \right) = 0 \xrightarrow{\pi^{t+1}} \frac{1}{\pi} \sum_i y_i^t = \frac{1}{1-\pi} \sum_i (1-y_i^t)$$

$$\rightarrow m\pi^{t+1} = \sum_i y_i^t \rightarrow \pi^{t+1} = \frac{\sum_i y_i^t}{m} \quad p_r^{t+1} = \frac{\sum_i x_i y_i^t}{\sum_i y_i^t}$$

$$p_b^{t+1} = \frac{\sum_i x_i - \sum_i x_i y_i^t}{m - \sum_i y_i^t}$$

4-

$$P(x_i | \mu, \Sigma) = \frac{1}{(2\pi)^{d/2} |\Sigma|^{1/2}} \exp\left(-\frac{1}{2} (x_i - \mu)^T \Sigma^{-1} (x_i - \mu)\right)$$

$$\mathcal{L} = P(X | \mu, \Sigma) = \prod_{i=1}^N P(x_i | \mu, \Sigma)$$

$$\log(y/b) = \log a - \log b$$

$$\log \mathcal{L} = \sum_i \log P(x_i | \mu, \Sigma) = \sum_i \left[ -\frac{d}{2} \log(2\pi) - \frac{1}{2} \log |\Sigma| - \frac{1}{2} (x_i - \mu)^T \Sigma^{-1} (x_i - \mu) \right] =$$

$$= -N \frac{d}{2} \log(2\pi) - \frac{N}{2} \log |\Sigma| - \frac{1}{2} \sum_i (x_i - \mu)^T \Sigma^{-1} (x_i - \mu)$$

$$\frac{\partial \log \mathcal{L}}{\partial \mu} = -\frac{1}{2} \sum_i \frac{\partial}{\partial \mu} \left[ (x_i - \mu)^T \Sigma^{-1} (x_i - \mu) \right] = -\frac{1}{2} \sum_i \left[ -2 \Sigma^{-1} (x_i - \mu) \right] =$$

$$= \sum_i \Sigma^{-1} (x_i - \mu) = \Sigma^{-1} \sum_i (x_i - \mu) = 0 \rightarrow \sum_i x_i = n\mu$$

$$\mu = \frac{1}{n} \sum_i x_i$$

b)

$$\pi_1 \mathcal{N}(x | \mu, \Sigma) + \pi_2 \mathcal{N}(x | \mu, \Sigma) = (\pi_1 + \pi_2) \dots$$

$$c) \quad P(z=1|x) \propto \pi_1 \mathcal{N}(x|\mu_1, \sigma^2)$$

$$P(z=2|x) \propto \pi_2 \mathcal{N}(x|\mu_2, \sigma^2)$$

$$\pi_1 \mathcal{N}(x|\mu_1, \sigma^2) = \pi_2 \mathcal{N}(x|\mu_2, \sigma^2) \rightarrow \pi_1 e^{-\frac{(x-\mu_1)^2}{2\sigma^2}} = \pi_2 e^{-\frac{(x-\mu_2)^2}{2\sigma^2}}$$

$$\rightarrow \ln \pi_1 - \frac{(x-\mu_1)^2}{2\sigma^2} = \ln \pi_2 - \frac{(x-\mu_2)^2}{2\sigma^2}$$

$$\ln \pi_1 - \ln \pi_2 = \frac{(x-\mu_1)^2 - (x-\mu_2)^2}{2\sigma^2} = \frac{-2\mu_1 x + 2\mu_2 x + \mu_1^2 - \mu_2^2}{2\sigma^2} = 2\sigma^2 \ln\left(\frac{\pi_1}{\pi_2}\right)$$

$$\rightarrow 2x^* (\mu_2 - \mu_1) = 2\sigma^2 \ln(\pi_1/\pi_2) - (\mu_1^2 - \mu_2^2)$$

$$\rightarrow x^* = \frac{\mu_1 + \mu_2}{2} + \frac{\sigma^2}{\mu_2 - \mu_1} \ln(\pi_1/\pi_2)$$